WebAssembly/Wasm_Base_Defs.thy
@@ -658,6 +658,19 @@ definition store_serialise_vec :: "storeop_vec \<Rightarrow> v128 \<Rightarrow> 
 definition cl_type :: "cl \<Rightarrow> tf" where
   "cl_type cl = (case cl of Func_native _ tf _ _ \<Rightarrow> tf | Func_host tf _ \<Rightarrow> tf)"
 
+definition tb_tf :: "inst \<Rightarrow> tb \<Rightarrow> tf" where
+  "tb_tf inst tb = (case tb of
+                      Tbf i \<Rightarrow> (inst.types inst)!i
+                    | Tbv (Some t) \<Rightarrow> ([] _> [t])
+                    | Tbv None \<Rightarrow> ([] _> []))"
+
+definition tb_tf_t :: "t_context \<Rightarrow> tb \<Rightarrow> tf option" where
+  "tb_tf_t \<C> tb = (case tb of
+                      Tbf i \<Rightarrow> let tfs = (types_t \<C>) in
+                               if i < length tfs then Some (tfs!i) else None
+                    | Tbv (Some t) \<Rightarrow> Some ([] _> [t])
+                    | Tbv None \<Rightarrow> Some ([] _> []))"
+
 definition rglob_is_mut :: "global \<Rightarrow> bool" where
   "rglob_is_mut g = (g_mut g = T_mut)"
 
